theories/Lambda.v
@@ -1,0 +1,46 @@
+Require Import Autosubst.Autosubst.
+Require Import Coq.Relations.Relation_Definitions.
+
+(* The ordinary λ-calculus *)
+(* ----------------------- *)
+
+Inductive λ: Type :=
+| Var (x: var)
+| Lam (t: {bind λ})
+| App (s t: λ).
+
+(* autosubst sorcery *)
+(* ----------------- *)
+
+Instance Ids_λ : Ids λ. derive. Defined.
+Instance Rename_λ : Rename λ. derive. Defined.
+Instance Subst_λ : Subst λ. derive. Defined.
+Instance SubstLemmas_λ : SubstLemmas λ. derive. Defined.
+
+(* beta reduction *)
+(* -------------- *) 
+
+Inductive step : relation λ :=
+| Step_Beta s s' t : s' = s.[t .: ids] ->
+                     step (App (Lam s) t) s'
+| Step_Abs s s' : step s s' ->
+                  step (Lam s) (Lam s')
+| Step_App1 s s' t: step s s' ->
+                    step (App s t) (App s' t)
+| Step_App2 s t t': step t t' ->
+                    step (App s t) (App s t').
+
+(* typing rules *)
+(* ------------ *)
+
+Require Import SimpleTypes.
+
+Inductive sequent (Γ: var->type) : λ -> type -> Prop := 
+| Ax (x: var) (A: type) :
+  Γ x = A -> sequent Γ (Var x) A
+
+| Intro (t: λ) (A B: type) :
+  sequent (A .: Γ) t B -> sequent Γ (Lam t) (Arr A B)
+                                 
+| Elim (s t: λ) (A B: type) :
+  sequent Γ s (Arr A B) -> sequent Γ t A -> sequent Γ (App s t) B.
