theories/SimpleTypes.v
@@ -1,0 +1,4 @@
+(* Simple Types *)
+(* ------------ *)
+
+Inductive type: Type := Base | Arr : type -> type -> type.
